theories/Bug.v
@@ -1,0 +1,27 @@
+From Equations Require Import Equations.
+
+Inductive expr :=
+with subst :=
+| S_id : subst
+| S_shift : subst
+| S_cons : expr -> subst -> subst
+| S_comp : subst -> subst -> subst.
+
+Equations f : subst -> subst -> subst :=
+f (S_comp S_shift s1) _ := s1 ;
+f s1 s2 := S_comp s1 s2.
+
+Lemma f_incorrect s1 s2 : 
+  f (S_comp S_id s1) s2 = S_comp (S_comp S_id s1) s1.
+Proof. reflexivity. Qed.
+
+Equations g : subst -> subst -> subst :=
+g (S_comp S_shift s1) _ := s1 ;
+g x y := S_comp x y.
+
+Lemma g_correct s1 s2 : 
+  g (S_comp S_id s1) s2 = S_comp (S_comp S_id s1) s2.
+Proof. reflexivity. Qed.
+
+
+
